Haskell/SGElemTys.hs
@@ -22,7 +22,7 @@ sgety_set = [Einh, Ewander, Eder] ++ [e d | e<-[Ecomp, Erel], d<-[Duni, Dbi]]
 -- Order which dictates allowed inheritance relations 
 nty_lti:: SGNTy->SGNTy->Bool
 nty_lti nt1 nt2 = ((nt2 == Nenum) `iff` (nt1 == Nval)) && ((nt1 == Nvirt) `implies` (nt2 == Nvirt)) && ((nt1 == Nabst) `implies` (nt2 `elem` [Nvirt, Nabst, Nprxy]))
-    &&  (not $ nt1 `elem` [Nprxy, Nenum]) && nt2 /= Nopt
+    &&  (not $ nt1 `elem` [Nprxy, Nenum, Nopt]) && nt2 /= Nopt
 
 -- Ordering used to state refinement relations
 nty_leqr:: SGNTy->SGNTy->Bool
