Isabelle/Fragmenta/Fragmenta_Frs.thy
@@ -9,31 +9,1035 @@ begin
 
 (*Fragments*)      
 record Fr = 
-  sg :: "SGr"
+  fsg :: "SGr"
+  esr :: "E set"
+  sr :: "E \<rightharpoonup> V"
   tr :: "E \<rightharpoonup> V"
 
-(*Set of all fragments*)
-definition is_fr :: "Fr \<Rightarrow> bool"
-where
-  "is_fr F \<equiv> True"
+definition consF::"SGr\<Rightarrow>E set\<Rightarrow>(E \<rightharpoonup> V)\<Rightarrow>(E \<rightharpoonup> V)\<Rightarrow>Fr"
+  where 
+  "consF sg es s t = \<lparr>fsg = sg, esr = es, sr = s, tr = t\<rparr>"
 
-definition fr_set :: "Fr set"
+(* Empty Fragment*)
+definition emptyF :: "Fr"
 where
-  "fr_set \<equiv> {F. is_fr F}"
-
-(* Defines the empty Fr*)
-definition emptyFr :: "Fr"
-where
-  "emptyFr \<equiv> \<lparr>sg = emptySG, tr = empty\<rparr>"
+  "emptyF \<equiv> consF emptySG {} Map.empty Map.empty"
 
 lemma Fr_eq: 
-  shows "(F1 = F2) \<longleftrightarrow> sg F1 = sg F2 \<and> tr F1 = tr F2 \<and> Fr.more F1 = Fr.more F2"
+  shows "(F1 = F2) \<longleftrightarrow> fsg F1 = fsg F2 \<and> esr F1 = esr F2
+    \<and> sr F1 = sr F2 \<and> tr F1 = tr F2 
+    \<and> Fr.more F1 = Fr.more F2"
     by (auto)
 
-(*Target function with directed references*)
-definition tgtr :: "'a Fr_scheme \<Rightarrow> E \<rightharpoonup> V"
+(*Local edges*)
+definition flEs :: "'a Fr_scheme \<Rightarrow> E set"
 where
-  "tgtr F \<equiv> tgt (sg F) ++ (tr F)"
+  "flEs F \<equiv> Es (fsg F)"
+
+(*All edges*)
+definition fEs :: "'a Fr_scheme \<Rightarrow> E set"
+where
+  "fEs F \<equiv> flEs F \<union> esr F"
+
+(*Local nodes*)
+definition flNs :: "'a Fr_scheme \<Rightarrow> V set"
+where
+  "flNs F \<equiv> Ns (fsg F)"
+
+(*Referenced nodes*)
+definition fRNs :: "'a Fr_scheme \<Rightarrow> V set"
+where
+  "fRNs F \<equiv> ran (tr F)"
+
+(*Fragment nodes*)
+definition fNs :: "'a Fr_scheme \<Rightarrow> V set"
+where
+  "fNs F \<equiv> flNs F \<union> fRNs F"
+
+(*Source function with directed references*)
+definition srcF :: "'a Fr_scheme \<Rightarrow> E \<rightharpoonup> V"
+where
+  "srcF F \<equiv> src (fsg F) ++ (sr F)"
+
+(*Target function with directed references*)
+definition tgtF :: "'a Fr_scheme \<Rightarrow> E \<rightharpoonup> V"
+where
+  "tgtF F \<equiv> tgt (fsg F) ++ (tr F)"
+
+definition wf_fz :: "'a Fr_scheme \<Rightarrow> bool"
+where
+  "wf_fz F \<equiv> wf_sg (fsg F) 
+    \<and> (esr F) \<subseteq> E_A 
+    \<and> (esr F) \<inter> (flEs F) = {}
+    \<and> fbij_on (sr F) (esr F) (NsP (fsg F))
+    \<and> ftotal_on (tr F) (esr F) (V_A - NsO (fsg F))"
+
+lemma wf_fz_wf_sg:
+  assumes "wf_fz F"
+  shows "wf_sg (fsg F)"
+  using assms by (simp add: wf_fz_def)
+
+lemma wf_fz_sr_bij:
+  assumes "wf_fz F"
+  shows "fbij_on (sr F) (esr F) (NsP (fsg F))"
+  using assms by (simp add: wf_fz_def)
+
+lemma wf_fz_disj_esr_fles:
+  assumes "wf_fz F"
+  shows "(esr F) \<inter> (flEs F) = {}"
+  using assms by (simp add: wf_fz_def)
+
+lemma wf_fz_esr_sub_EA:
+  assumes "wf_fz F"
+  shows "(esr F) \<subseteq> E_A"
+  using assms by (simp add: wf_fz_def)
+
+lemma wf_fz_tr_ftotal: 
+  assumes "wf_fz F"
+  shows "ftotal_on (tr F) (esr F) (V_A)"
+  using assms by (simp add: wf_fz_def)
+
+definition disj_fs::"'a Fr_scheme \<Rightarrow>'a Fr_scheme\<Rightarrow>bool" 
+  where
+  "disj_fs F1 F2 \<equiv> disjoint [flNs F1, flNs F2] \<and> disjoint [fEs F1, fEs F2]"
+
+lemma disj_fs_imp_disj_Gs:
+  assumes "wf_fz F1" and "wf_fz F2" and "disj_fs F1 F2"
+  shows "disjGs (fsg F1) (fsg F2)"
+  using assms disj_V_E wf_fz_wf_sg[of F1] wf_sg_wf_g[of "fsg F1"]
+    wf_fz_wf_sg[of F2] wf_sg_wf_g[of "fsg F2"]
+  by (auto simp add: disjGs_def disj_fs_def flNs_def fEs_def 
+      flEs_def  wf_g_def)
+
+definition disj_fsL::"'a Fr_scheme list \<Rightarrow>bool" 
+  where
+  "disj_fsL Fs \<equiv> disjGsL (map fsg Fs) \<and> disjoint(map esr Fs)"
+
+(*References Graph*)
+definition refsG :: "'a Fr_scheme \<Rightarrow> Gr"
+where
+  "refsG F \<equiv> consG (NsP (fsg F) \<union> (fRNs F)) (esr F) (sr F) (tr F)"
+
+lemma Ns_refsG[simp]: "Ns (refsG F) = NsP (fsg F) \<union> (fRNs F)"
+  by (auto simp add: refsG_def consG_def)
+
+lemma Es_refsG[simp]: "Es (refsG F) = esr F"
+  by (simp add: refsG_def consG_def)
+
+lemma src_refsG[simp]: "src (refsG F) = (sr F)"
+  by (simp add: refsG_def consG_def)
+
+lemma tgt_refsG[simp]: "tgt (refsG F) = (tr F)"
+  by (simp add: refsG_def consG_def)
+
+definition refEOf ::"'a Fr_scheme \<Rightarrow>V\<Rightarrow>E option"
+  where
+  "refEOf F \<equiv> \<lambda> v. if v \<in> NsP( fsg F) then (Some (the_elem ((sr F) -`{Some v}))) else None"
+
+lemma one_e_in_dom_sr:
+  assumes "wf_fz F" and "v \<in> NsP( fsg F)"
+  shows "\<exists>!e. sr F e = Some v"
+  proof (rule ccontr)
+    assume h: "\<nexists>!e. sr F e = Some v"
+    have "v \<in> ran (sr F)"
+      using assms wf_fz_sr_bij[of F]
+      by (simp add: fbij_on_def)
+    hence "\<exists> e. sr F e = Some v" by (simp add: ran_def)
+    then show "False"
+      using h assms wf_fz_sr_bij[of F]
+      by (force simp add: fbij_on_def finj_on_def Map_Extra.injective_def)
+  qed
+
+lemma refEOfIsFLE:
+  assumes "wf_fz F" and "v \<in> NsP( fsg F)"
+  shows "the (refEOf F v) \<in> (esr F)"
+proof -
+  show ?thesis
+  proof (simp add: assms(2) refEOf_def)
+    have h1: "\<exists>!e. sr F e = Some v"
+      using assms one_e_in_dom_sr[of F v] by simp
+    from h1 obtain e where "sr F e = Some v" by auto
+    hence h2: "the_elem (sr F -` {Some v}) = e"
+      using the1_equality[of "\<lambda> e. sr F e = Some v" "e"] h1
+      by (auto simp add: the_elem_def vimage_def)
+    have "e \<in> dom (sr F)" 
+      using \<open>sr F e = Some v\<close> by (simp add: dom_def)
+    then show "the_elem (sr F -` {Some v}) \<in> esr F"
+      using h2 assms wf_fz_sr_bij[of F] 
+      by (simp add: fbij_on_def finj_on_def ftotal_on_def)
+  qed
+qed
+
+lemma dom_refEOf_eq_NsP:
+  assumes "wf_fz F"
+  shows "dom(refEOf F) = NsP( fsg F)"
+  by (auto simp add: refEOf_def domIff subsetI split: if_splits)
+
+lemma ran_refEOf_eq_esr:
+  assumes "wf_fz F"
+  shows "ran(refEOf F) = esr F"
+proof
+  show "ran (refEOf F) \<subseteq> esr F"
+    by (smt (verit, best) assms domI dom_refEOf_eq_NsP mem_Collect_eq option.sel ran_def refEOfIsFLE subsetI)
+next
+  show "esr F \<subseteq> ran (refEOf F)"
+  proof
+    fix e
+    assume "e \<in> esr F"
+    hence "e \<in> dom (sr F)"
+      using assms wf_fz_sr_bij[of F]
+      by (simp add: fbij_on_def finj_on_def ftotal_on_def)
+    then obtain v where "(sr F) e = Some v" by auto
+    hence "v \<in> NsP (fsg F)"
+      using assms wf_fz_sr_bij[of F]
+      by (force simp add: fbij_on_def ranI)
+    hence "\<exists>!e. sr F e = Some v"
+      using assms one_e_in_dom_sr[of F v] by simp
+    hence "the_elem (sr F -` {Some v}) = e"
+      using the1_equality[of "\<lambda> e. sr F e = Some v" "e"]
+      \<open>sr F e = Some v\<close>
+      by (auto simp add: the_elem_def vimage_def)
+    then show "e \<in> ran (refEOf F)"
+      using \<open>v \<in> NsP (fsg F)\<close>
+      by (auto simp add: refEOf_def ran_def)
+  qed
+qed
+
+lemma sr_F_the_refEOf_eq_v:
+  assumes "wf_fz F" and "v \<in> NsP( fsg F)"
+  shows "sr F (the (refEOf F v)) = Some v"
+proof (simp add: assms(2) refEOf_def vimage_def)
+  have h1: "\<exists>!e. sr F e = Some v"
+      using assms one_e_in_dom_sr[of F v] by simp
+  from h1 obtain e where "sr F e = Some v" by auto
+  hence h2: "the_elem {x. sr F x = Some v} = e"
+    using the1_equality[of "\<lambda> e. sr F e = Some v" "e"] h1
+    by (auto simp add: the_elem_def vimage_def)
+  then show "sr F (the_elem {x. sr F x = Some v}) = Some v"
+    using \<open>sr F e = Some v\<close> by auto
+qed
+
+(*References partial function, used in fragment resolution*)
+definition refs :: "'a Fr_scheme \<Rightarrow> (V \<rightharpoonup> V)"
+  where
+  "refs F \<equiv> (\<lambda>v. if v \<in> NsP( fsg F) then  (tr F) (the (refEOf F v)) else None)"
+
+lemma dom_refsF:
+  assumes "wf_fz F"
+  shows "dom (refs F) = NsP( fsg F)"
+proof
+  show "dom (refs F) \<subseteq> NsP (fsg F)"
+    by (simp add: refs_def domIff subset_iff)
+next
+  show "NsP (fsg F) \<subseteq> dom (refs F)"
+  proof
+    fix v
+    assume "v \<in> NsP (fsg F)"
+    then show "v \<in> dom (refs F)"
+    using assms wf_fz_tr_ftotal[of F] refEOfIsFLE[of F]
+    by (auto simp add: refs_def domIff ftotal_on_def)
+  qed
+qed
+
+lemma ran_refsF:
+  assumes "wf_fz F"
+  shows "ran (refs F) \<subseteq> V_A"
+  using assms wf_fz_tr_ftotal[of F]
+  by (auto simp add: refs_def subset_eq ftotal_on_def ran_def)
+
+lemma Domain_refsG_eq_NsP:
+  assumes "wf_fz F"
+  shows "Domain ((refsG F)\<^sup>\<Leftrightarrow>) = NsP( fsg F)"
+proof
+  show "Domain ((refsG F)\<^sup>\<Leftrightarrow>) \<subseteq> NsP( fsg F)"
+  proof
+    fix v
+    assume "v \<in> Domain ((refsG F)\<^sup>\<Leftrightarrow>)"
+    hence "v \<in> ran(sr F)"
+      by (auto simp add: relG_def adjacent_def ran_def)
+    then show "v \<in> NsP (fsg F)"
+      using assms wf_fz_sr_bij[of F] 
+      by (simp add: fbij_on_def)
+  qed
+next
+  show "NsP (fsg F) \<subseteq> Domain ((refsG F)\<^sup>\<Leftrightarrow>)"
+  proof
+    fix v
+    assume "v \<in> NsP (fsg F)"
+    hence "v \<in> ran(sr F)"
+      using assms wf_fz_sr_bij[of F] 
+      by (auto simp add: ran_def fbij_on_def)
+    then obtain e where "e \<in> esr F \<and> sr F e = Some v"
+      using assms wf_fz_sr_bij[of F]
+      by (auto simp add: ran_def fbij_on_def finj_on_def ftotal_on_def)
+    from \<open>e \<in> esr F \<and> sr F e = Some v\<close> obtain v' where "tr F e = Some v'"
+      using assms wf_fz_tr_ftotal[of F]
+      by (auto simp add: ftotal_on_def ran_def)
+    show "v \<in> Domain ((refsG F)\<^sup>\<Leftrightarrow>)"
+      using \<open>e \<in> esr F \<and> sr F e = Some v\<close> \<open>tr F e = Some v'\<close>
+      by (auto simp add: Domain_iff relG_def adjacent_def)
+  qed
+qed
+
+lemma refsF_eq_refsG_rel:
+  assumes "wf_fz F"
+  shows "pfunToRel (refs F) = (refsG F)\<^sup>\<Leftrightarrow>"
+proof 
+  show "pfunToRel (refs F) \<subseteq> (refsG F)\<^sup>\<Leftrightarrow>"
+  proof (rule subrelI)
+    fix v v'
+    assume h: "(v, v') \<in> pfunToRel (refs F)"
+    hence "v \<in> NsP (fsg F)"
+      using assms dom_refsF
+      by (auto simp add: pfunToRel_iff)
+    hence "\<exists> e. e = the (refEOf F v) \<and> sr F e = Some v \<and> tr F e = Some v'"
+      using h assms 
+      by (auto simp add: refs_def pfunToRel_def sr_F_the_refEOf_eq_v)
+    then show "(v, v') \<in> (refsG F)\<^sup>\<Leftrightarrow>"
+      using \<open>v \<in> NsP (fsg F)\<close> adjacent_def assms 
+        refEOfIsFLE relG_def by fastforce
+  qed
+next
+  show "(refsG F)\<^sup>\<Leftrightarrow> \<subseteq> pfunToRel (refs F)"
+  proof (rule subrelI)
+    fix v v'
+    assume h: "(v, v') \<in> (refsG F)\<^sup>\<Leftrightarrow>"
+    hence "v \<in> NsP (fsg F)"
+    using assms Domain_refsG_eq_NsP
+    by (auto)
+    hence "v \<in> ran(sr F)"
+      using assms wf_fz_sr_bij[of F] 
+      by (auto simp add: ran_def fbij_on_def)
+    from \<open>v \<in> ran(sr F)\<close> obtain e where "e \<in> esr F \<and> sr F e = Some v"
+      using assms wf_fz_sr_bij[of F]
+      by (auto simp add: ran_def fbij_on_def finj_on_def ftotal_on_def)
+    have "tr F e = Some v'"
+      using assms wf_fz_tr_ftotal[of F] h  \<open>e \<in> esr F \<and> sr F e = Some v\<close>
+      \<open>v \<in> NsP (fsg F)\<close> one_e_in_dom_sr
+      by (auto simp add: ftotal_on_def relG_def adjacent_def)
+    have "the (refEOf F v) = e"
+      using assms \<open>e \<in> esr F \<and> sr F e = Some v\<close> \<open>v \<in> NsP (fsg F)\<close>
+       one_e_in_dom_sr[of F v]
+      by (auto simp add: refEOf_def vimage_def the_elem_def)
+    show "(v, v') \<in> pfunToRel (refs F)"
+      using \<open>tr F e = Some v'\<close> \<open>e \<in> esr F \<and> sr F e = Some v\<close> 
+      \<open>v \<in> NsP (fsg F)\<close> \<open>the (refEOf F v) = e\<close>
+      by (auto simp add: pfunToRel_iff refs_def)
+  qed
+qed
+
+(*Fragments union*)
+definition cupF :: "Fr \<Rightarrow> Fr \<Rightarrow> Fr" (infixl "\<union>\<^sub>F" 100)
+where
+  "F1 \<union>\<^sub>F F2 \<equiv> \<lparr>fsg =  (fsg F1) USG (fsg F2), esr = esr F1 \<union> esr F2,
+    sr = sr F1 ++ sr F2, tr = tr F1 ++ tr F2\<rparr>"
+
+lemma fsg_UF[simp]: "fsg (F1 \<union>\<^sub>F F2) = (fsg F1) USG (fsg F2)"
+  by (simp add: cupF_def)
+
+lemma esr_UF[simp]: "esr (F1 \<union>\<^sub>F F2) = esr F1 \<union> esr F2"
+  by (simp add: cupF_def)
+
+lemma sr_UF[simp]: "sr (F1 \<union>\<^sub>F F2) = sr F1 ++ sr F2"
+  by (simp add: cupF_def)
+
+lemma tr_UF[simp]: "tr (F1 \<union>\<^sub>F F2) = tr F1 ++ tr F2"
+  by (simp add: cupF_def)
+
+(*In most cases, '++' equates to union as fragments are disjoint*)
+
+(* builds union of a set of fragments*)
+primrec bUF :: "Fr list \<Rightarrow>Fr" ("\<Union>\<^sub>F") 
+where
+  bUF_base: "\<Union>\<^sub>F [] = emptyF" |
+  bUF_induct: "\<Union>\<^sub>F (F#Fs) = F \<union>\<^sub>F (\<Union>\<^sub>F Fs)"
+
+lemma refEOf_map_add_f:
+  assumes "wf_fz F1" and "wf_fz F2"  and "disj_fs F1 F2" 
+    and "v \<in> NsP (fsg F1)"
+  shows "(refEOf F1 ++ refEOf F2) v = refEOf F1 v"
+    using assms wf_fz_wf_sg[of F1] wf_fz_wf_sg[of F2]
+         dom_refEOf_eq_NsP[of F1] dom_refEOf_eq_NsP[of F2] 
+         map_add_disj_domf[of "refEOf F1" "refEOf F2" v]
+         NsP_sub_Ns[of "fsg F1"] NsP_sub_Ns[of "fsg F2"]
+    by (force simp add: disj_fs_def flNs_def fEs_def flEs_def)
+
+lemma tr_map_addrefEOf_f:
+  assumes "wf_fz F1" and "wf_fz F2"  and "disj_fs F1 F2" 
+    and "v \<in> NsP (fsg F1)"
+  shows "(tr F1 ++ tr F2) (the (refEOf F1 v)) = tr F1 (the (refEOf F1 v))"
+proof-
+  have "dom (tr F1) \<inter> dom(tr F2) = {}"
+      using assms wf_fz_tr_ftotal[of F1] wf_fz_tr_ftotal[of F2]
+      by (auto simp add:  disj_fs_def ftotal_on_def fEs_def)
+  have "the (refEOf F1 v) \<in> dom (tr F1)"
+    using assms wf_fz_tr_ftotal[of F1] refEOfIsFLE[of F1 v]
+    by (simp add: ftotal_on_dom)
+  show ?thesis
+    using assms \<open>dom (tr F1) \<inter> dom(tr F2) = {}\<close> 
+    \<open>the (refEOf F1 v) \<in> dom (tr F1)\<close> 
+    map_add_disj_domf[of "tr F1" "tr F2" "the (refEOf F1 v)"] 
+    by simp
+qed
+
+lemma refEOf_UF:
+  assumes "wf_fz F1" and "wf_fz F2" and "disj_fs F1 F2"
+  shows "refEOf (F1 \<union>\<^sub>F F2) = (refEOf F1)++(refEOf F2)"
+proof -
+  have "dom (sr F1) \<inter> dom(sr F2) = {}"
+      using assms wf_fz_sr_bij[of F1] wf_fz_sr_bij[of F2]
+      by (auto simp add:  disj_fs_def fbij_on_def finj_on_def 
+          ftotal_on_def fEs_def)
+  have "ran (sr F1) \<inter> ran(sr F2) = {}"
+      using assms wf_fz_sr_bij[of F1] wf_fz_sr_bij[of F2]
+      wf_fz_wf_sg[of F1] wf_fz_wf_sg[of F2]
+      NsP_sub_Ns[of "fsg F1"] NsP_sub_Ns[of "fsg F2"]
+      by (auto simp add:  disj_fs_def fbij_on_def fEs_def flNs_def)
+  show ?thesis
+  proof
+    fix v
+    show "refEOf (F1 \<union>\<^sub>F F2) v = (refEOf F1 ++ refEOf F2) v"
+    proof (case_tac "v \<in> NsP (fsg F1 USG fsg F2)")
+      assume "v \<in> NsP (fsg F1 USG fsg F2)"
+      hence "v \<in> NsP (fsg F1) \<or> v \<in> NsP (fsg F2)"
+        using assms wf_fz_wf_sg[of F1] wf_fz_wf_sg[of F2] 
+        by (simp add: disj_fs_imp_disj_Gs NsP_USG)
+      then show "refEOf (F1 \<union>\<^sub>F F2) v = (refEOf F1 ++ refEOf F2) v"
+      proof
+        assume "v \<in> NsP (fsg F1)"
+        hence "v \<in> ran(sr F1)"
+          using assms wf_fz_sr_bij[of F1] 
+          by (auto simp add: ran_def fbij_on_def)
+        show "refEOf (F1 \<union>\<^sub>F F2) v = (refEOf F1 ++ refEOf F2) v"
+          using \<open>v \<in> NsP (fsg F1 USG fsg F2)\<close>
+            \<open>dom (sr F1) \<inter> dom(sr F2) = {}\<close>
+            \<open>ran (sr F1) \<inter> ran(sr F2) = {}\<close>
+            \<open>v \<in> ran(sr F1)\<close> \<open>v \<in> NsP (fsg F1)\<close>
+            assms vimage_disj_ran_1[of "sr F1" "sr F2" v]
+          by (simp only: refEOf_map_add_f)
+            (auto simp add: refEOf_def split: option.splits)
+      next
+        assume "v \<in> NsP (fsg F2)"
+        hence "v \<in> ran(sr F2)"
+          using assms wf_fz_sr_bij[of F2] 
+          by (auto simp add: ran_def fbij_on_def)
+        have h: "(refEOf F1 ++ refEOf F2) v = refEOf F2 v"
+          using \<open>v \<in> NsP (fsg F2)\<close> assms(2)
+            \<open>dom (sr F1) \<inter> dom(sr F2) = {}\<close>
+            \<open>ran (sr F1) \<inter> ran(sr F2) = {}\<close>
+          by (simp add: dom_refEOf_eq_NsP map_add_dom_app_simps)
+        show "refEOf (F1 \<union>\<^sub>F F2) v = (refEOf F1 ++ refEOf F2) v"
+          using \<open>v \<in> NsP (fsg F1 USG fsg F2)\<close> \<open>v \<in> NsP (fsg F2)\<close>
+          vimage_disj_ran_2[of "sr F1" "sr F2" v]
+          \<open>v \<in> ran(sr F2)\<close> \<open>dom (sr F1) \<inter> dom(sr F2) = {}\<close>
+            \<open>ran (sr F1) \<inter> ran(sr F2) = {}\<close>
+          by (simp only: h)
+          (auto simp add: refEOf_def split: option.splits)
+      qed
+    next
+      assume "v \<notin> NsP (fsg F1 USG fsg F2)"
+      hence "v \<notin> NsP (fsg F1) \<and> v \<notin> NsP (fsg F2)"
+        using assms
+        by (simp add: NsP_USG disj_fs_imp_disj_Gs wf_fz_wf_sg)
+      hence h: "(refEOf F1 ++ refEOf F2) v = None"
+        by (simp add: refEOf_def)
+      then show "refEOf (F1 \<union>\<^sub>F F2) v = (refEOf F1 ++ refEOf F2) v"
+        using \<open>v \<notin> NsP (fsg F1 USG fsg F2)\<close>
+        by (simp add: h)(simp add: refEOf_def)
+    qed
+  qed
+qed
+
+(*References relation restricted to local references*)
+definition refsL :: "'a Fr_scheme \<Rightarrow> (V \<rightharpoonup> V)"
+  where
+  "refsL F \<equiv> (refs F) \<rhd>\<^sub>m (flNs F)"
+
+(*Unresolved references edges of a fragment*)
+definition uRefEs :: "'a Fr_scheme \<Rightarrow> E set"
+  where
+  "uRefEs F \<equiv> dom ((sr F) \<unrhd>\<^sub>m dom (refsL F))"
+
+(*Resolves a fragment's SG*)
+definition fresolveSG ::  "'a Fr_scheme \<Rightarrow> SGr" ("(\<Odot>\<^sup>S\<^sup>G_)" [1000] 999)
+  where
+  "\<Odot>\<^sup>S\<^sup>G F = (fsg F) \<odot>\<^sup>S\<^sup>G (refsL F)"
+
+(*Resolves a fragment*)
+definition fresolve ::"'a Fr_scheme \<Rightarrow> Fr" ("(\<Odot>_)" [1000] 999)
+  where
+  "\<Odot> F = consF (\<Odot>\<^sup>S\<^sup>G F) (uRefEs F) ((sr F) |` (uRefEs F)) ((tr F) |` (uRefEs F))"
+
+definition wf_fa::"'a Fr_scheme \<Rightarrow>bool"
+where
+  "wf_fa F \<equiv> wf_fz F \<and> acyclicGr (refsG F)"
+
+definition wf_f::"'a Fr_scheme \<Rightarrow>bool"
+where
+  "wf_f F \<equiv> wf_fa F \<and> wf_sg (\<Odot>\<^sup>S\<^sup>G F)"
+
+definition refsLocal::"'a Fr_scheme \<Rightarrow>bool"
+  where
+  "refsLocal F \<equiv> fRNs F \<subseteq> flNs F"
+
+definition wf_tf::"'a Fr_scheme \<Rightarrow>bool"
+  where
+  "wf_tf F \<equiv> wf_fa F \<and> refsLocal F \<and> wf_tsg (\<Odot>\<^sup>S\<^sup>G F)"
+
+lemma wf_fa_wf_fz:
+  assumes "wf_fa F"
+  shows "wf_fz F"
+  using assms
+  by (simp add: wf_fa_def)
+
+lemma wf_f_wf_fa:
+  assumes "wf_f F"
+  shows "wf_fa F"
+  using assms
+  by (simp add: wf_f_def)
+
+lemma wf_f_wf_sg:
+  assumes "wf_f F"
+  shows "wf_sg (fsg F)"
+  using assms
+  by (simp add: wf_f_def wf_fa_def wf_fz_def)
+
+lemma wf_tf_wf_fa:
+  assumes "wf_tf F"
+  shows "wf_fa F"
+  using assms
+  by (simp add: wf_tf_def)
+
+lemma wf_tf_refsLocal:
+  assumes "wf_tf F"
+  shows "refsLocal F"
+  using assms by (simp add: wf_tf_def)
+
+
+definition frefs_in::"'a Fr_scheme \<Rightarrow>'a Fr_scheme \<Rightarrow> bool" (infixl "\<subseteq>\<^sup>r\<^sup>s" 100) 
+  where
+  "F1 \<subseteq>\<^sup>r\<^sup>s F2 \<equiv> ran (tr F1) \<inter> fNs F2 \<noteq> {}"
+
+definition refs_from_to::"'a Fr_scheme \<Rightarrow>'a Fr_scheme \<Rightarrow> bool" (infixl "\<Rightarrow>\<^sup>r\<^sup>s" 100)
+  where
+  "F1 \<Rightarrow>\<^sup>r\<^sup>s F2 \<equiv> F1 \<subseteq>\<^sup>r\<^sup>s F2 \<and> \<not>(F2 \<subseteq>\<^sup>r\<^sup>s F1)"
+
+lemma flEs_UF: 
+  shows "flEs (F1 \<union>\<^sub>F F2) = flEs F1 \<union> flEs F2"
+  by (simp add: cupF_def flEs_def disj_fs_def 
+      wf_fz_def ftotal_on_def cupSG_def) 
+
+lemma flNs_UF: 
+  shows "flNs (F1 \<union>\<^sub>F F2) = flNs F1 \<union> flNs F2"
+  by (simp add: cupF_def flNs_def disj_fs_def 
+      wf_fz_def ftotal_on_def cupSG_def) 
+
+lemma fRNs_UF: 
+  assumes "wf_fz F1" and "wf_fz F2" and "disj_fs F1 F2"
+  shows "fRNs (F1 \<union>\<^sub>F F2) = fRNs F1 \<union> fRNs F2"
+  using assms
+  ran_map_add[of "tr F1" "tr F2"]
+  by (auto simp add: cupF_def fRNs_def disj_fs_def 
+      wf_fz_def ftotal_on_def fEs_def)  
+
+lemma refsG_UF:
+  assumes "wf_fa F1" and "wf_fa F2" and "disj_fs F1 F2"
+  shows "refsG (F1 \<union>\<^sub>F F2) = refsG F1 UG refsG F2"
+  using assms wf_fa_wf_fz[of F1]  wf_fa_wf_fz[of F2] 
+    wf_fz_wf_sg[of F1] wf_fz_wf_sg[of F2]
+    NsP_USG[of "fsg F1" "fsg F2"] fRNs_UF[of F1 F2]
+    disj_fs_imp_disj_Gs
+  by (auto simp add: refsG_def disj_fs_def cupG_def consG_def)
+
+lemma wf_refsG:
+  assumes "wf_fa F"
+  shows "wf_g (refsG F)"
+  using assms wf_fa_wf_fz[of F] wf_fz_wf_sg[of F]
+    wf_fz_wf_sg[of F] wf_sg_wf_g[of "fsg F"]
+proof (simp add: refsG_def wf_g_def consG_def)
+  apply_end(rule conjI)
+  show "NsP (fsg F) \<subseteq> V_A"
+    using assms wf_fa_wf_fz[of F] wf_fz_wf_sg[of F]
+    wf_sg_wf_g[of "fsg F"] 
+    NsP_sub_Ns[of "fsg F"]
+    by (auto simp add: wf_g_def wf_fz_def)
+next
+  apply_end(rule conjI)
+  show "fRNs F \<subseteq> V_A"
+    using assms wf_fa_wf_fz[of F]
+    by (simp add: wf_fz_def fRNs_def ftotal_on_def)
+next
+  apply_end(rule conjI)
+  show "esr F \<subseteq> E_A"
+    using assms wf_fa_wf_fz[of F]
+    by (simp add: wf_fz_def)
+next
+  apply_end(rule conjI)
+  show "ftotal_on (tr F) (esr F) (NsP (fsg F) \<union> fRNs F)"
+    using assms wf_fa_wf_fz[of F] wf_fz_wf_sg[of F]
+    NsP_sub_Ns[of "fsg F"]
+    by (simp add: ftotal_on_def consG_def wf_fz_def 
+        fbij_on_def finj_on_def fRNs_def)
+next
+  show "ftotal_on (sr F) (esr F) (NsP (fsg F) \<union> fRNs F)"
+  using assms wf_fa_wf_fz[of F] wf_fz_wf_sg[of F]
+    NsP_sub_Ns[of "fsg F"]
+    by (simp add: ftotal_on_def consG_def wf_fz_def 
+        fbij_on_def finj_on_def fRNs_def)
+qed
+
+lemma wf_fa_acyclicGr_refsG:
+  assumes "wf_fa F"
+  shows "acyclicGr (refsG F)"
+  using assms by (simp add: wf_fa_def)
+
+lemma disj_fs_imp_disjEsGs_RefsGs:
+  assumes "disj_fs F1 F2"
+  shows "disjEsGs (refsG F1) (refsG F2)"
+  using assms
+  by (auto simp add: refsG_def consG_def fRNs_def disjEsGs_def 
+      disj_fs_def flNs_def fEs_def flEs_def)
+
+lemma Domain_RefsG_eq_NsPSG:
+  assumes "wf_fa F"
+  shows "Domain ((refsG F)\<^sup>\<Leftrightarrow>) = NsP (fsg F)"
+proof
+  show "Domain ((refsG F)\<^sup>\<Leftrightarrow>) \<subseteq> NsP (fsg F)"
+  using assms wf_fa_wf_fz[of F] wf_fz_wf_sg[of F]
+    wf_fz_sr_bij[of F] 
+    by (auto simp add: fbij_on_def relG_def adjacent_def refsG_def
+        consG_def finj_on_def ftotal_on_def intro: ranI)
+next
+  show " NsP (fsg F) \<subseteq> Domain ((refsG F)\<^sup>\<Leftrightarrow>)"
+  proof
+    fix x
+    assume "x \<in> NsP (fsg F)"
+    hence "x \<in> ran (sr F)" 
+      using assms wf_fz_sr_bij[of F] 
+      by (simp add: wf_fa_def fbij_on_def)
+    then obtain e where "e \<in> esr F \<and> sr F e = Some x" 
+      using assms wf_fa_wf_fz[of F] wf_fz_sr_bij[of F] 
+      by (auto simp add: ran_def fbij_on_def finj_on_def ftotal_on_def)
+    then obtain v where "tr F e = Some v" 
+      using assms wf_fa_wf_fz[of F] wf_fz_tr_ftotal[of F]
+      by (auto simp add: ftotal_on_def)
+    show "x \<in> Domain ((refsG F)\<^sup>\<Leftrightarrow>)"
+      using \<open>e \<in> esr F \<and> sr F e = Some x\<close> \<open>tr F e = Some v\<close>
+      by (auto simp add: relG_def adjacent_def refsG_def consG_def)
+  qed
+qed
+
+lemma Range_RefsG_eq_fRNs:
+  assumes "wf_fa F"
+  shows "Range ((refsG F)\<^sup>\<Leftrightarrow>) = fRNs F"
+proof
+  show "Range ((refsG F)\<^sup>\<Leftrightarrow>) \<subseteq> fRNs F"
+  using assms wf_fa_wf_fz[of F] wf_fz_wf_sg[of F]
+    wf_fz_sr_bij[of F] 
+    by (auto simp add: fbij_on_def relG_def adjacent_def refsG_def
+        consG_def fRNs_def intro: ranI)
+next
+  show "fRNs F \<subseteq> Range ((refsG F)\<^sup>\<Leftrightarrow>)"
+  proof
+    fix x
+    assume "x \<in> fRNs F"
+    then obtain e where "e \<in> esr F \<and> tr F e = Some x" 
+      using assms wf_fa_wf_fz[of F] wf_fz_tr_ftotal[of F]
+      by (auto simp add: fRNs_def ran_def ftotal_on_def)
+    hence "e \<in> dom (sr F)" 
+      using assms wf_fa_wf_fz[of F] wf_fz_sr_bij[of F]
+      by (auto simp add: fbij_on_def finj_on_def 
+          ftotal_on_def)
+    then obtain v where "sr F e = Some v" 
+      using assms 
+      by (auto simp add: domD)
+    then show "x \<in> Range ((refsG F)\<^sup>\<Leftrightarrow>)"
+      using \<open>e \<in> esr F \<and> tr F e = Some x\<close>
+      by (auto simp add: refsG_def consG_def fRNs_def relG_def
+          adjacent_def)
+  qed
+qed
+
+lemma refs_from_to_implies:
+  assumes "wf_fa F2" and "F1 \<Rightarrow>\<^sup>r\<^sup>s F2"
+  shows "(fRNs F2) \<inter> (fNs F1) = {}"
+proof (rule ccontr)
+  assume h: "(fRNs F2) \<inter> (fNs F1) \<noteq> {}"
+  then obtain x where "x \<in> (fRNs F2) \<inter> (fNs F1)"
+    by auto
+  hence "x \<in> fRNs F2" by auto
+  hence "x \<notin> fNs F1"
+    using assms(2) by (auto simp add: refs_from_to_def frefs_in_def
+        fRNs_def fNs_def)
+  then show "False"
+    using \<open>x \<in> (fRNs F2) \<inter> (fNs F1)\<close> by auto
+qed
+  
+lemma acyclic_UF: 
+  assumes "wf_fa F1" and "wf_fa F2" and "disj_fs F1 F2" and "F1 \<Rightarrow>\<^sup>r\<^sup>s F2"
+  shows "acyclicGr (refsG (F1 \<union>\<^sub>F F2)) = (acyclicGr (refsG F1) \<and> acyclicGr (refsG F2))"
+proof
+  assume "acyclicGr (refsG (F1 \<union>\<^sub>F F2))"
+  then show "acyclicGr (refsG F1) \<and> acyclicGr (refsG F2)"
+    using assms wf_refsG[of F1] wf_refsG[of F2] 
+      disj_fs_imp_disjEsGs_RefsGs[of F1 F2] 
+    by (simp add: acyclic_Gr_UG_disj_imp_acylic_Grs refsG_UF)
+next
+  apply_end(clarsimp)
+  assume h1: "acyclicGr (refsG F1)" and h2: "acyclicGr (refsG F2)"
+  from h1 have "acyclic ((refsG F1)\<^sup>\<Leftrightarrow>)" 
+    by (simp add: acyclic_Gr_iff_acyclic_relG)
+  from h2 have "acyclic ((refsG F2)\<^sup>\<Leftrightarrow>)" 
+    by (simp add: acyclic_Gr_iff_acyclic_relG)
+  have "Domain ((refsG F1)\<^sup>\<Leftrightarrow>) \<inter> Domain ((refsG F2)\<^sup>\<Leftrightarrow>) = {}"
+    using assms wf_fa_wf_fz[of F1] wf_fa_wf_fz[of F2] 
+     wf_fz_wf_sg[of F1] wf_fz_wf_sg[of F2] 
+     NsP_sub_Ns[of "fsg F1"] NsP_sub_Ns[of "fsg F2"]
+     Domain_RefsG_eq_NsPSG[of F1] Domain_RefsG_eq_NsPSG[of F2]
+     ns_disj_Ga_Gb[of "fsg F1" "fsg F2"]
+     disj_fs_imp_disj_Gs[of F1 F2]
+    by (auto simp add: disj_fs_def flNs_def)
+  have "Range ((refsG F2)\<^sup>\<Leftrightarrow>) \<inter> Domain ((refsG F1)\<^sup>\<Leftrightarrow>) = {}"
+  proof (rule ccontr)
+    assume "Range ((refsG F2)\<^sup>\<Leftrightarrow>) \<inter> Domain ((refsG F1)\<^sup>\<Leftrightarrow>) \<noteq> {}"
+    then obtain x where "x \<in> Range ((refsG F2)\<^sup>\<Leftrightarrow>) \<inter> Domain ((refsG F1)\<^sup>\<Leftrightarrow>)"
+      by auto
+    hence "x \<in> (fRNs F2)" 
+      using assms(2) 
+      by (simp add: Range_RefsG_eq_fRNs)
+    have "x \<in> (fNs F1)"
+      using \<open>x \<in> Range ((refsG F2)\<^sup>\<Leftrightarrow>) \<inter> Domain ((refsG F1)\<^sup>\<Leftrightarrow>)\<close> 
+      assms(1) assms(2) NsP_sub_Ns[of "fsg F1"] 
+      wf_fa_wf_fz[of F1] wf_fz_wf_sg[of F1]
+      by (auto simp add: Domain_RefsG_eq_NsPSG fNs_def
+          flNs_def)
+    then show "False"
+      using assms(2) assms(4) refs_from_to_implies[of F2 F1] 
+      \<open>x \<in> (fRNs F2)\<close> 
+      by auto
+  qed
+  hence "acyclic (((refsG F1)\<^sup>\<Leftrightarrow>) \<union> ((refsG F2)\<^sup>\<Leftrightarrow>))"
+    using \<open>Domain ((refsG F1)\<^sup>\<Leftrightarrow>) \<inter> Domain ((refsG F2)\<^sup>\<Leftrightarrow>) = {}\<close>
+    \<open>acyclic ((refsG F1)\<^sup>\<Leftrightarrow>)\<close> \<open>acyclic ((refsG F2)\<^sup>\<Leftrightarrow>)\<close> 
+    by (simp add: acyclic_Un)
+  then show "acyclicGr (refsG (F1 \<union>\<^sub>F F2))"
+    using assms relG_UG wf_refsG[of F1] wf_refsG[of F2]
+    disj_fs_imp_disjEsGs_RefsGs[of F1 F2]
+  by (simp add: refsG_UF acyclic_Gr_iff_acyclic_relG 
+       relG_UG)
+qed
+
+lemma wfz_UF: 
+  assumes "wf_fz F1" and "wf_fz F2" and "disj_fs F1 F2"
+    and "F1 \<Rightarrow>\<^sup>r\<^sup>s F2"
+  shows "wf_fz (F1 \<union>\<^sub>F F2)"
+proof (simp add: wf_fz_def)
+  apply_end(rule conjI)
+  show "wf_sg (fsg F1 USG fsg F2)"
+    using assms wf_fz_wf_sg[of F1] wf_fz_wf_sg[of F2]
+    disj_fs_imp_disj_Gs[of F1 F2]
+    by (simp add: is_wf_sg_Un disj_fs_def)
+next
+  apply_end(rule conjI)
+  show "esr F1 \<subseteq> E_A"
+    using assms(1) by (simp add: wf_fz_def)
+next
+  apply_end(rule conjI)
+  show "esr F2 \<subseteq> E_A"
+    using assms(2) by (simp add: wf_fz_def)
+next
+  apply_end(rule conjI)
+  have h: "(esr F1 \<union> esr F2) \<inter> flEs (F1 \<union>\<^sub>F F2) =
+    (esr F1 \<inter> flEs (F1 \<union>\<^sub>F F2)) \<union> (esr F2 \<inter> flEs (F1 \<union>\<^sub>F F2))" 
+    by auto
+  show "(esr F1 \<union> esr F2) \<inter> flEs (F1 \<union>\<^sub>F F2) = {}"
+  proof (rule ccontr)
+    assume "(esr F1 \<union> esr F2) \<inter> flEs (F1 \<union>\<^sub>F F2) \<noteq> {}"
+    hence "(esr F1 \<inter> flEs (F1 \<union>\<^sub>F F2)) \<union> (esr F2 \<inter> flEs (F1 \<union>\<^sub>F F2)) \<noteq> {}"
+      using h by auto
+    then obtain x where "x \<in> (esr F1 \<inter> flEs (F1 \<union>\<^sub>F F2)) \<union> (esr F2 \<inter> flEs (F1 \<union>\<^sub>F F2))"
+      by auto
+    hence "x \<in> (esr F1 \<inter> flEs (F1 \<union>\<^sub>F F2)) \<or> x \<in> (esr F2 \<inter> flEs (F1 \<union>\<^sub>F F2))" 
+    using assms(1) assms(2)
+    by (simp add: flEs_UF wf_fz_def)
+  then show "False" 
+    using flEs_UF[of F1 F2] assms(1) assms(2)
+      assms(3)
+      wf_fz_disj_esr_fles[of F1] disj_fs_imp_disj_Gs[of F1 F2]
+      wf_fz_disj_esr_fles[of F2]
+      by (auto simp add: disj_fs_def flEs_def fEs_def)
+  qed
+next
+  apply_end(rule conjI)
+  have "disjoint [esr F1, esr F2, NsP (fsg F1), NsP (fsg F2)]"
+    using assms wf_fz_wf_sg[of F1] wf_fz_wf_sg[of F2] 
+      NsP_sub_Ns[of "fsg F1"]  NsP_sub_Ns[of "fsg F2"] 
+      wf_fz_disj_esr_fles[of F1] wf_fz_disj_esr_fles[of F2]
+      wf_fz_esr_sub_EA[of F1] wf_fz_esr_sub_EA[of F2]
+      disj_V_E wf_sg_wf_g[of "fsg F1"] wf_sg_wf_g[of "fsg F2"]
+    by (force simp add: disj_fs_def flNs_def flEs_def fEs_def
+        wf_g_def)
+  show "fbij_on (sr F1 ++ sr F2) (esr F1 \<union> esr F2)
+     (NsP (fsg F1 USG fsg F2))"
+    using assms wf_fz_sr_bij[of F1]
+       wf_fz_sr_bij[of F2] wf_fz_wf_sg[of F1]
+       wf_fz_wf_sg[of F2] disj_fs_imp_disj_Gs[of F1 F2]
+       \<open>disjoint [esr F1, esr F2, NsP (fsg F1), NsP (fsg F2)]\<close>
+      fbij_on_dist_map_add[of "sr F1" "esr F1" "NsP (fsg F1)" 
+        "sr F2" "esr F2" "NsP (fsg F2)"] 
+    by (auto simp add: NsP_USG)
+next
+  have "esr F1 \<inter> esr F2 = {}"
+    using assms(3) by (auto simp add:  disj_fs_def fEs_def flEs_def)
+  then show " ftotal_on (tr F1 ++ tr F2) (esr F1 \<union> esr F2) V_A"
+    using assms wf_fz_tr_ftotal[of F1]
+    wf_fz_tr_ftotal[of F2] 
+    ftotal_on_map_add[of "tr F1" "esr F1" "V_A" "tr F2" "esr F2" "V_A"] 
+    by (simp)
+qed
+
+lemma wfa_UF: 
+  assumes "wf_fa F1" and "wf_fa F2" and "disj_fs F1 F2"
+    and "F1 \<Rightarrow>\<^sup>r\<^sup>s F2"
+  shows "wf_fa (F1 \<union>\<^sub>F F2)"
+proof (simp add: wf_fa_def)
+  apply_end(rule conjI)
+  show "wf_fz (F1 \<union>\<^sub>F F2)"
+    using assms wf_fa_wf_fz[of F1] wf_fa_wf_fz[of F2]
+    by (simp add: wfz_UF)
+next
+  show "acyclicGr (refsG (F1 \<union>\<^sub>F F2))"
+    using assms  wf_fa_acyclicGr_refsG[of F1]
+      wf_fa_acyclicGr_refsG[of F2]
+    by (simp add: acyclic_UF)
+qed
+
+lemma wf_tf_ran_refsF_Ns_SG:
+  assumes "wf_tf F"
+  shows "ran (refs F) \<subseteq> Ns (fsg F)"
+  using assms wf_tf_refsLocal[of F]
+  by (auto simp add: refs_def fRNs_def refsLocal_def 
+      flNs_def subset_eq ran_def split: if_splits)
+
+lemma dom_refs_disj:
+  assumes "wf_fz F1" and "wf_fz F2" and h3: "disj_fs F1 F2"
+  shows "dom (refs F1) \<inter> dom (refs F2) = {}"
+  using assms wf_fz_wf_sg[of F1] wf_fz_wf_sg[of F2]  
+    dom_refsF[of F1] dom_refsF[of F2] 
+    disj_fs_imp_disj_Gs[of F1 F2]
+    NsP_sub_Ns[of "fsg F1"] NsP_sub_Ns[of "fsg F2"]
+  by (auto simp add: disjGs_def)
+  
+lemma refs_UF:
+  assumes "wf_f F1" and "wf_f F2" and h3: "disj_fs F1 F2"
+  shows "refs (F1 \<union>\<^sub>F F2) = refs F1 ++ refs F2"
+proof
+  fix v
+  show "refs (F1 \<union>\<^sub>F F2) v = (refs F1 ++ refs F2) v"
+  proof (case_tac "v \<in> NsP (fsg F1 USG fsg F2)")
+    assume "v \<in> NsP (fsg F1 USG fsg F2)"
+    hence "v \<in> NsP (fsg F1) \<or> v \<in> NsP (fsg F2)"
+      using assms wf_f_wf_fa[of F1] wf_f_wf_fa[of F2] 
+        wf_fa_wf_fz[of F1] wf_fa_wf_fz[of F2] 
+        wf_fz_wf_sg[of F1] wf_fz_wf_sg[of F2] 
+        NsP_USG[of "fsg F1" "fsg F2"]
+      by (simp add: refs_def disj_fs_imp_disj_Gs)
+    then show "refs (F1 \<union>\<^sub>F F2) v = (refs F1 ++ refs F2) v"
+    proof
+      assume "v \<in> NsP (fsg F1)"
+      have h: "(refs F1 ++ refs F2) v = refs F1 v"
+        using assms dom_refsF[of F1] wf_f_wf_fa[of F1] 
+          wf_fa_wf_fz[of F1] wf_f_wf_fa[of F2] 
+          wf_fa_wf_fz[of F2] dom_refs_disj[of F1 F2]
+          map_add_disj_domf[of "refs F1" "refs F2" v]
+          \<open>v \<in> NsP (fsg F1)\<close>
+        by (simp)
+      show "refs (F1 \<union>\<^sub>F F2) v = (refs F1 ++ refs F2) v"
+        using assms wf_f_wf_fa[of F1] wf_fa_wf_fz[of F1]
+        wf_f_wf_fa[of F2] wf_fa_wf_fz[of F2]
+        \<open>v \<in> NsP (fsg F1 USG fsg F2)\<close> \<open>v \<in> NsP (fsg F1)\<close>
+        by (simp add: h)
+          (simp add: refs_def refEOf_UF refEOf_map_add_f
+            tr_map_addrefEOf_f split: option.splits)
+    next
+      assume "v \<in> NsP (fsg F2)"
+      hence "v \<in> dom (refs F2)"
+        using assms dom_refsF[of F2] 
+          wf_f_wf_fa[of F2] wf_fa_wf_fz[of F2] 
+        by auto
+      hence h: "(refs F1 ++ refs F2) v = refs F2 v"
+        by (simp add: map_add_dom_app_simps(1))
+      have "v \<in> dom(refEOf F2)"
+        using \<open>v \<in> NsP (fsg F2)\<close> assms(2)
+        by (simp add:  dom_refEOf_eq_NsP wf_f_wf_fa wf_fa_wf_fz)
+      have "the (refEOf F2 v) \<in> dom (tr F2)"
+        using assms(2) wf_f_wf_fa[of F2] wf_fa_wf_fz[of F2]
+          \<open>v \<in> NsP (fsg F2)\<close> refEOfIsFLE[of F2 v]
+          wf_fz_tr_ftotal[of F2]
+        by (simp add: ftotal_on_dom)
+      then show "refs (F1 \<union>\<^sub>F F2) v = (refs F1 ++ refs F2) v"
+        using assms wf_f_wf_fa[of F1] wf_fa_wf_fz[of F1]
+        wf_f_wf_fa[of F2] wf_fa_wf_fz[of F2]
+          \<open>v \<in> NsP (fsg F1 USG fsg F2)\<close> \<open>v \<in> NsP (fsg F2)\<close>
+          \<open>v \<in> dom(refEOf F2)\<close>
+        by (simp add: h)
+          (simp add: refs_def refEOf_UF map_add_dom_app_simps(1))
+    qed
+  next
+    assume "v \<notin> NsP (fsg F1 USG fsg F2)"
+    hence "v \<notin> NsP (fsg F1) \<and> v \<notin> NsP (fsg F2)"
+      using assms wf_f_wf_fa[of F1] wf_fa_wf_fz[of F1] 
+       wf_fz_wf_sg[of F1] wf_f_wf_fa[of F2] wf_fa_wf_fz[of F2] 
+       wf_fz_wf_sg[of F2] disj_fs_imp_disj_Gs[of F1 F2]
+      by (simp add: NsP_USG)
+    then show "refs (F1 \<union>\<^sub>F F2) v = (refs F1 ++ refs F2) v"
+      using \<open>v \<notin> NsP (fsg F1 USG fsg F2)\<close>
+      by (simp add: refs_def map_add_dom_app_simps(3) domIff)
+  qed
+qed
+
+lemma wff_refsL_partial:
+  assumes "wf_f F" 
+  shows "fpartial_on (refsL F) (NsP (fsg F)) (Ns (fsg F))"
+proof (simp add: fpartial_on_def)
+  apply_end(rule conjI)
+  show "dom (refsL F) \<subseteq> NsP (fsg F)"
+    using assms wf_f_wf_fa[of F] wf_fa_wf_fz[of F]
+    dom_refsF[of F] dom_mrres_sub_dom[of "refs F" "flNs F"]
+    by (simp add: refsL_def)
+next
+  show "ran (refsL F) \<subseteq> Ns (fsg F)"
+    using assms mrres_ran_sub1[of "refs F" "flNs F"]
+    by (simp add: refsL_def mrres_ran_sub2 flNs_def)
+qed
+
+
+lemma wf_ufs_refsL_partial:
+  assumes "wf_f F1" and  "wf_f F2"  and "disj_fs F1 F2" 
+  shows "fpartial_on (refsL (F1 \<union>\<^sub>F F2)) (NsP (fsg (F1 \<union>\<^sub>F F2))) (Ns (fsg (F1 \<union>\<^sub>F F2)))"
+proof (simp add: fpartial_on_def)
+  apply_end(rule conjI)
+  have "dom (refs F2) \<union> dom (refs F1) \<subseteq> NsP (fsg F1) \<union> NsP (fsg F2)"
+    using assms(1) assms(2)
+    by (simp add:  dom_refsF wf_f_wf_fa wf_fa_wf_fz)
+  then show "dom (refsL (F1 \<union>\<^sub>F F2)) \<subseteq> NsP (fsg F1 USG fsg F2)"
+    using assms wf_f_wf_fa[of F1] wf_fa_wf_fz[of F1] 
+      wf_fz_wf_sg[of F1] wf_f_wf_fa[of F2] wf_fa_wf_fz[of F2] 
+      wf_fz_wf_sg[of F2] disj_fs_imp_disj_Gs[of F1 F2] 
+      dom_mrres_sub_dom[of "refs F1 ++ refs F2" "flNs F1 \<union> flNs F2"]
+    by (force simp add: refsL_def NsP_USG refs_UF flNs_UF)
+next
+  show "ran (refsL (F1 \<union>\<^sub>F F2)) \<subseteq> Ns (fsg F1) \<union> Ns (fsg F2)"
+    using assms 
+      mrres_ran_sub1[of "refs F1 ++ refs F2" "(flNs F1 \<union> flNs F2)"]
+    by (simp add: refsL_def refs_UF flNs_UF flNs_def)
+qed
+
+lemma wf_sg_fresolveSG:
+  assumes "wf_f F1" and "wf_f F2" and "disj_fs F1 F2" 
+    and "F1 \<Rightarrow>\<^sup>r\<^sup>s F2"
+  shows "wf_sg(\<Odot>\<^sup>S\<^sup>G(F1 \<union>\<^sub>F F2))"
+proof (simp add: wf_sg_def)
+  apply_end(rule conjI)
+  show "wf_g (\<Odot>\<^sup>S\<^sup>G(F1 \<union>\<^sub>F F2))"
+    using assms(1) assms(2) assms(3) wf_f_wf_fa[of F1]
+       wf_fa_wf_fz[of F1] wf_fz_wf_sg[of F1]
+      wf_f_wf_fa[of F2]
+       wf_fa_wf_fz[of F2] wf_fz_wf_sg[of F2] disj_fs_imp_disj_Gs[of F1 F2]
+      wf_g_subsumeSG[of "fsg F1 USG fsg F2" "refsL (F1 \<union>\<^sub>F F2)"]
+      is_wf_sg_Un[of "fsg F1" "fsg F2"]
+      wf_ufs_refsL_partial
+    by (simp add: fresolveSG_def )
+next
+  apply_end(rule conjI)
+  show "ftotal_on (nty (\<Odot>\<^sup>S\<^sup>G(F1 \<union>\<^sub>F F2))) (Ns (\<Odot>\<^sup>S\<^sup>G(F1 \<union>\<^sub>F F2)))
+     SGNT_set"
+    using assms(1) assms(2) assms(3) wf_f_wf_fa[of F1]
+       wf_fa_wf_fz[of F1] wf_fz_wf_sg[of F1]
+       wf_f_wf_fa[of F2]
+       wf_fa_wf_fz[of F2] wf_fz_wf_sg[of F2]
+       disj_fs_imp_disj_Gs[of F1 F2]
+       is_wf_sg_Un[of "fsg F1" "fsg F2"]
+       ftotal_on_nty_subsumeSG[of "fsg F1 USG fsg F2" "refsL (F1 \<union>\<^sub>F F2)"]
+       wf_ufs_refsL_partial
+    by (simp add: fresolveSG_def )
+next
+  apply_end(rule conjI)
+  show "ftotal_on (ety (\<Odot>\<^sup>S\<^sup>G(F1 \<union>\<^sub>F F2))) (Es (\<Odot>\<^sup>S\<^sup>G(F1 \<union>\<^sub>F F2)))
+     SGET_set"
+    using assms(1) assms(2) assms(3) wf_f_wf_fa[of F1]
+       wf_fa_wf_fz[of F1] wf_fz_wf_sg[of F1]
+       wf_f_wf_fa[of F2]
+       wf_fa_wf_fz[of F2] wf_fz_wf_sg[of F2]
+       disj_fs_imp_disj_Gs[of F1 F2]
+       is_wf_sg_Un[of "fsg F1" "fsg F2"]
+       ftotal_on_ety_subsumeSG[of "fsg F1 USG fsg F2" "refsL (F1 \<union>\<^sub>F F2)"]
+       wf_ufs_refsL_partial
+    by (simp add: fresolveSG_def )
+next
+  apply_end(rule conjI)
+  show "ftotal_on (srcma (\<Odot>\<^sup>S\<^sup>G(F1 \<union>\<^sub>F F2))) (EsC (\<Odot>\<^sup>S\<^sup>G(F1 \<union>\<^sub>F F2)))
+     MultC_set"
+  using assms(1) assms(2) assms(3) wf_f_wf_fa[of F1]
+       wf_fa_wf_fz[of F1] wf_fz_wf_sg[of F1]
+       wf_f_wf_fa[of F2]
+       wf_fa_wf_fz[of F2] wf_fz_wf_sg[of F2]
+       disj_fs_imp_disj_Gs[of F1 F2]
+       is_wf_sg_Un[of "fsg F1" "fsg F2"]
+       ftotal_on_srcma_subsumeSG[of "fsg F1 USG fsg F2" "refsL (F1 \<union>\<^sub>F F2)"]
+       wf_ufs_refsL_partial
+  by (simp add: fresolveSG_def )
+next
+  apply_end(rule conjI)
+  show "ftotal_on (tgtm (\<Odot>\<^sup>S\<^sup>G(F1 \<union>\<^sub>F F2))) (EsC (\<Odot>\<^sup>S\<^sup>G(F1 \<union>\<^sub>F F2)))
+     MultC_set"
+  using assms(1) assms(2) assms(3) wf_f_wf_fa[of F1]
+       wf_fa_wf_fz[of F1] wf_fz_wf_sg[of F1]
+       wf_f_wf_fa[of F2]
+       wf_fa_wf_fz[of F2] wf_fz_wf_sg[of F2]
+       disj_fs_imp_disj_Gs[of F1 F2]
+       is_wf_sg_Un[of "fsg F1" "fsg F2"]
+       ftotal_on_tgtm_subsumeSG[of "fsg F1 USG fsg F2" "refsL (F1 \<union>\<^sub>F F2)"]
+       wf_ufs_refsL_partial
+  by (simp add: fresolveSG_def )
+next
+  apply_end(rule conjI)
+  show "dom (db (\<Odot>\<^sup>S\<^sup>G(F1 \<union>\<^sub>F F2))) = EsD (\<Odot>\<^sup>S\<^sup>G(F1 \<union>\<^sub>F F2))"
+  using assms(1) assms(2) assms(3) wf_f_wf_fa[of F1]
+       wf_fa_wf_fz[of F1] wf_fz_wf_sg[of F1]
+       wf_f_wf_fa[of F2]
+       wf_fa_wf_fz[of F2] wf_fz_wf_sg[of F2]
+       disj_fs_imp_disj_Gs[of F1 F2]
+       is_wf_sg_Un[of "fsg F1" "fsg F2"]
+       dom_db_eq_EsD_subsumeSG[of "fsg F1 USG fsg F2" "refsL (F1 \<union>\<^sub>F F2)"]
+       wf_ufs_refsL_partial
+  by (simp add: fresolveSG_def )
+next
+  apply_end(rule conjI)
+  show "multsOk (\<Odot>\<^sup>S\<^sup>G(F1 \<union>\<^sub>F F2))"
+  using assms(1) assms(2) assms(3) wf_f_wf_fa[of F1]
+       wf_fa_wf_fz[of F1] wf_fz_wf_sg[of F1]
+       wf_f_wf_fa[of F2]
+       wf_fa_wf_fz[of F2] wf_fz_wf_sg[of F2]
+       disj_fs_imp_disj_Gs[of F1 F2]
+       is_wf_sg_Un[of "fsg F1" "fsg F2"]
+       multsOk_subsumeSG[of "fsg F1 USG fsg F2" "refsL (F1 \<union>\<^sub>F F2)"]
+       wf_ufs_refsL_partial
+  by (simp add: fresolveSG_def )
+next
+  
+lemma wf_U_Frs_1: 
+  assumes "wf_f F1" and "wf_f F2" and "disj_fs F1 F2" 
+    and "F1 \<Rightarrow>\<^sup>r\<^sup>s F2"
+  shows "wf_f (F1 \<union>\<^sub>F F2)"
+proof (simp add: wf_f_def)
+  apply_end(rule conjI)
+  show " wf_fa (F1 \<union>\<^sub>F F2)"
+    using assms by (simp add: wf_f_def wfa_UF)
+next
+  show "wf_sg (\<Odot>\<^sup>S\<^sup>G(F1 \<union>\<^sub>F F2))"
+    
+qed
 
 (*Yields the fragment's graph but filled with the references of proxies*)
 definition withRsG :: "'a Fr_scheme \<Rightarrow> Gr"
@@ -53,27 +1057,10 @@ lemma src_withRsG[simp]: "src (withRsG F) = src (sg F)"
 lemma tgt_withRsG[simp]: "tgt (withRsG F) = tgtr F"
   by (simp add: withRsG_def)
 
-(*Yields graph of proxies and their references*)
-definition refsG :: "'a Fr_scheme \<Rightarrow> Gr"
-where
-  "refsG F \<equiv> restrict (withRsG F) (EsRP (sg F))"
-
-lemma Ns_refsG[simp]: "Ns (refsG F) = rst_Ns (withRsG F) (EsRP (sg F))"
-  by (auto simp add: refsG_def)
-
-lemma Es_refsG[simp]: "Es (refsG F) = Es (sg F) \<inter> (EsRP (sg F))"
-  by (simp add: refsG_def)
-
-lemma src_refsG[simp]: "src (refsG F) = rst_fun (EsRP (sg F)) (src (sg F))"
-  by (simp add: refsG_def)
-
-lemma tgt_refsG[simp]: "tgt (refsG F) = rst_fun (EsRP (sg F)) (tgtr F)"
-  by (simp add: refsG_def)
-
 (*Yields inheritance graph together with proxies and their references*)
 definition inhRefsG :: "'a Fr_scheme \<Rightarrow> Gr"
 where
-  "inhRefsG F \<equiv> inhG (sg F) UG refsG F"
+  "inhRefsG F \<equiv> inhG (fsg F) UG refsG F"
 
 lemma Ns_inhRefsG[simp]: "Ns (inhRefsG F) = rst_Ns (sg F) (EsI (sg F) - EsId (sg F)) 
   \<union> rst_Ns (withRsG F) (EsRP (sg F))"
@@ -209,18 +1196,7 @@ definition disjFs :: "Fr list \<Rightarrow> bool"
 where
   "disjFs Fs \<equiv> disjGsL (map sg Fs)"
 
-(*Fragments union*)
-definition cupF :: "Fr \<Rightarrow> Fr \<Rightarrow> Fr" (infixl "UF" 100)
-where
-  "F1 UF F2 \<equiv> \<lparr>sg =  (sg F1) USG (sg F2), tr = tr F1 ++ tr F2\<rparr>"
 
-lemma tr_UF[simp]: "tr (F1 UF F2) = tr F1 ++ tr F2"
-  by (simp add: cupF_def)
-
-lemma sg_UF[simp]: "sg (F1 UF F2) = (sg F1) USG (sg F2)"
-  by (simp add: cupF_def)
-
-(*Above '++' equates to union because fragments are disjoint*)
 
 lemma UF_sym: 
   assumes h1: "is_wf_fr F1" and h2: "is_wf_fr F2" and h3: "disjGs (sg F1) (sg F2)"
@@ -778,18 +1754,7 @@ lemma refsG_fr_Un_dist:
     qed
   qed
 
-lemma refs_UF:
-  assumes h1: "is_wf_fr F1" and h2: "is_wf_fr F2" and h3: "disjGs (sg F1) (sg F2)"
-  shows "refs (F1 UF F2) = refs F1 \<union> refs F2"
-  proof -
-    from h1 have h1a: "is_wf_g (refsG F1)" by (simp add: is_wf_refsG)
-    from h2 have h2a: "is_wf_g (refsG F2)" by (simp add: is_wf_refsG)
-    from h3 have h3a: "disjEsGs (sg F1) (sg F2)" by (simp add: disjGs_def  disjEsGs_def)
-    from h3a have h3b: "disjEsGs (refsG F1) (refsG F2)" 
-      by (auto simp add: disjEsGs_def)
-    show ?thesis
-    using assms h1a h2a h3b by (simp add: refs_def refsG_fr_Un_dist relOfGr_UG)
-  qed
+
 
 lemma refs_trcl_UF:
   assumes h1: "is_wf_fr F1" and h2: "is_wf_fr F2" and h3: "disjGs (sg F1) (sg F2)"
