Isabelle/Fragmenta/Fragmenta_SGElemTys.thy
@@ -36,7 +36,7 @@ definition ilt_NT::"SGNT \<Rightarrow> SGNT  \<Rightarrow> bool" (infixl "<\<^su
   "nt\<^sub>1 <\<^sub>N\<^sub>T nt\<^sub>2 \<equiv> nt\<^sub>2 = nenum \<longleftrightarrow> nt\<^sub>1 = nval
     \<and> nt\<^sub>1 = nvirt \<longrightarrow> nt\<^sub>2 = nvirt
     \<and> nt\<^sub>1 = nabst \<longrightarrow>  nt\<^sub>2 \<in> {nabst, nprxy, nvirt}
-    \<and> nt\<^sub>1 \<notin> {nprxy, nenum} \<and> nt\<^sub>2 \<noteq> nopt"
+    \<and> nt\<^sub>1 \<notin> {nprxy, nenum, nopt} \<and> nt\<^sub>2 \<noteq> nopt"
 
 (*Dictates allowed refinement relations between node types*)
 definition rleq_NT::"SGNT \<Rightarrow> SGNT  \<Rightarrow> bool" (infixl "\<le>\<^sub>N\<^sub>T" 100)
